src/common/Nemonuri.Ref.fst
@@ -1,0 +1,7 @@
+module Nemonuri.Ref
+
+type t = {
+  v: nat
+}
+
+let is_null (ref:t) : Tot bool = ref.v = 0
