src/common/Nemonuri.Refinement.Tot.fst
@@ -1,0 +1,10 @@
+module Nemonuri.Refinement.Tot
+
+open FStar.FunctionalExtensionality
+
+noeq
+type t (a:eqtype) = { predicate: a ^-> bool }
+
+let equal (#a:eqtype) (r1:t a) (r2:t a) = feq r1.predicate r2.predicate
+
+let refine (#a:eqtype) (r:t a) : Tot eqtype = x:a{r.predicate x}
