src/ecma335/Nemonuri.Ecma335.Metadata.Heap.fst
@@ -2,27 +2,40 @@ module Nemonuri.Ecma335.Metadata.Heap
 
 module M = Nemonuri.Ecma335.Metadata
 module Te = Nemonuri.Ecma335.Metadata.TableEntry
+module Ter = Nemonuri.Ecma335.Metadata.TableEntry.Refinement
 module S = FStar.Set
+module Ref = Nemonuri.Ref
 
 open Nemonuri.Ecma335.Metadata.Table
 open FStar.Tactics.Typeclasses
-
-//assume val string_data : Type0
-//assume val guid_data : Type0
 
 class emptyable (a:Type) = {
   is_empty : a -> bool
 }
 
-let is_indexing_empty (#data_t:Type) {| e : emptyable data_t |} (table:tablelike Te.t data_t) (te:Te.t) : Tot bool =
+let is_indexing_empty (#data_t:Type) {| e : emptyable data_t |} (table:tablelike Te.t data_t) (te:Te.t{has_id table te}) : Tot bool =
   match Te.is_null te with
   | true -> false
-  | false ->
-  match S.mem te table.id_set with
-  | false -> false
-  | true -> table.get_data te |> e.is_empty
+  | false -> table.get_data te |> e.is_empty
   
+//--- string ---
+type string_data = { ref:Ref.t }
 
-//instance tablelike_string_heap {| e : emptyable string_data |} : tablelike Te.string_heap_index string_data = {
-//  try_get_data = fun _ -> None
-//}
+instance emptyable_string : emptyable string_data = {
+  is_empty = fun str -> str.ref |> Ref.is_null
+}
+//---|
+
+//--- guid ---
+type guid_data = { ref:Ref.t }
+
+instance emptyable_guid : emptyable guid_data = {
+  is_empty = fun g -> g.ref |> Ref.is_null
+}
+//---|
+
+let is_indexing_empty_string (e:Ter.string_heap_index{not (is_null e)}) : Tot bool =
+  false // Todo: be specific
+
+let is_indexing_null_guid (e:guid_heap_index{not (is_null e)}) : Tot bool =
+  false // Todo: be specific
