src/ecma335/Nemonuri.Ecma335.Metadata.Table.fst
@@ -1,12 +1,15 @@
 module Nemonuri.Ecma335.Metadata.Table
 
 module M = Nemonuri.Ecma335.Metadata
-module S = FStar.Set
+module Rf = Nemonuri.Refinement.Tot
 
 open FStar.Tactics.Typeclasses
 
 class tablelike (id_t:eqtype) (data_t:Type) =
 {
-  id_set : S.set id_t;
-  get_data : x:id_t{S.mem x id_set} -> data_t
+  id_domain : Rf.t id_t;
+  get_data : (Rf.refine id_domain) -> data_t
 }
+
+let has_id (#id_t:eqtype) (#data_t:Type) (table: tablelike id_t data_t) (id:id_t) : Tot bool =
+  table.id_domain.predicate id
