src/ecma335/Nemonuri.Ecma335.Metadata.TableEntry.Refinement.fst
@@ -1,0 +1,16 @@
+module Nemonuri.Ecma335.Metadata.TableEntry.Refinement
+
+module M = Nemonuri.Ecma335.Metadata
+module Te = Nemonuri.Ecma335.Metadata.TableEntry
+module Rf = Nemonuri.Refinement.Tot
+module F = FStar.FunctionalExtensionality
+
+let string_heap_index : Rf.t Te.t = {
+  predicate = F.on Te.t Te.StringHeap?
+}
+
+let guid_heap_index : Rf.t Te.t = {
+  predicate = F.on Te.t Te.GuidHeap?
+}
+
+let assert_string_and_guid_indexes_are_distinct (s:Rf.refine string_heap_index) (g:Rf.refine guid_heap_index) = assert (~(s === g))
